format-version: 1.2
data-version: releases/2015-03-10
subsetdef: bgee_not_trusted "Terms that are considered not trusted by the Bgee team, related to assertions needing additional support."
default-namespace: cio
ontology: cio
owl-axioms: Prefix(owl:=<http://www.w3.org/2002/07/owl#>)\nPrefix(rdf:=<http://www.w3.org/1999/02/22-rdf-syntax-ns#>)\nPrefix(xml:=<http://www.w3.org/XML/1998/namespace>)\nPrefix(xsd:=<http://www.w3.org/2001/XMLSchema#>)\nPrefix(rdfs:=<http://www.w3.org/2000/01/rdf-schema#>)\n\n\nOntology(\nEquivalentClasses(<http://purl.obolibrary.org/obo/CIO_0000000> ObjectUnionOf(ObjectIntersectionOf(ObjectAllValuesFrom(<http://purl.obolibrary.org/obo/has_evidence_concordance> <http://purl.obolibrary.org/obo/CIO_0000043>) ObjectMinCardinality(2 <http://purl.obolibrary.org/obo/has_confidence_element> <http://purl.obolibrary.org/obo/CIO_0000040>) ObjectMinCardinality(0 <http://purl.obolibrary.org/obo/has_confidence_level> <http://purl.obolibrary.org/obo/CIO_0000028>) ObjectExactCardinality(1 <http://purl.obolibrary.org/obo/has_evidence_type_concordance> <http://purl.obolibrary.org/obo/CIO_0000041>) ObjectMaxCardinality(3 <http://purl.obolibrary.org/obo/has_confidence_element> <http://purl.obolibrary.org/obo/CIO_0000040>) ObjectMaxCardinality(1 <http://purl.obolibrary.org/obo/has_confidence_level> <http://purl.obolibrary.org/obo/CIO_0000028>)) ObjectIntersectionOf(ObjectAllValuesFrom(<http://purl.obolibrary.org/obo/has_evidence_concordance> <http://purl.obolibrary.org/obo/CIO_0000042>) ObjectMinCardinality(1 <http://purl.obolibrary.org/obo/has_confidence_element> <http://purl.obolibrary.org/obo/CIO_0000040>) ObjectMinCardinality(0 <http://purl.obolibrary.org/obo/has_confidence_level> <http://purl.obolibrary.org/obo/CIO_0000028>) ObjectExactCardinality(0 <http://purl.obolibrary.org/obo/has_evidence_type_concordance> <http://purl.obolibrary.org/obo/CIO_0000041>) ObjectMaxCardinality(2 <http://purl.obolibrary.org/obo/has_confidence_element> <http://purl.obolibrary.org/obo/CIO_0000040>) ObjectMaxCardinality(1 <http://purl.obolibrary.org/obo/has_confidence_level> <http://purl.obolibrary.org/obo/CIO_0000028>))))\nObjectPropertyDomain(<http://purl.obolibrary.org/obo/has_confidence_level> ObjectIntersectionOf(ObjectAllValuesFrom(<http://purl.obolibrary.org/obo/has_evidence_concordance> ObjectComplementOf(<http://purl.obolibrary.org/obo/CIO_0000035>)) <http://purl.obolibrary.org/obo/CIO_0000000>))\nObjectPropertyDomain(<http://purl.obolibrary.org/obo/has_evidence_type_concordance> ObjectIntersectionOf(ObjectAllValuesFrom(<http://purl.obolibrary.org/obo/has_evidence_concordance> <http://purl.obolibrary.org/obo/CIO_0000043>) <http://purl.obolibrary.org/obo/CIO_0000000>))\n)

[Term]
id: CIO:0000000
name: confidence information statement
def: "A statement providing information about the confidence in an assertion, meaning, an information about the level of certainty that an assertion is correct." [Bgee:fbb]
comment: Quality and confidence are distinct concepts: quality refers to the value of a source or of an annotation, whereas confidence refers to the level of certainty that an assertion is correct.
intersection_of: has_confidence_element CIO:0000040 {minCardinality="1"} ! confidence information element
intersection_of: has_confidence_element CIO:0000040 {maxCardinality="3"} ! confidence information element
intersection_of: has_confidence_level CIO:0000028 {minCardinality="0"} ! confidence level
intersection_of: has_confidence_level CIO:0000028 {maxCardinality="1"} ! confidence level
intersection_of: has_evidence_concordance CIO:0000032 {cardinality="1"} ! evidence concordance
intersection_of: has_evidence_type_concordance CIO:0000041 {minCardinality="0"} ! evidence type concordance
intersection_of: has_evidence_type_concordance CIO:0000041 {maxCardinality="1"} ! evidence type concordance
disjoint_from: CIO:0000040 ! confidence information element
relationship: has_confidence_element CIO:0000040 {minCardinality="1"} ! confidence information element
relationship: has_confidence_element CIO:0000040 {maxCardinality="3"} ! confidence information element
relationship: has_confidence_level CIO:0000028 {maxCardinality="1"} ! confidence level
relationship: has_confidence_level CIO:0000028 {minCardinality="0"} ! confidence level
relationship: has_evidence_concordance CIO:0000032 {cardinality="1"} ! evidence concordance
relationship: has_evidence_type_concordance CIO:0000041 {maxCardinality="1"} ! evidence type concordance
relationship: has_evidence_type_concordance CIO:0000041 {minCardinality="0"} ! evidence type concordance

[Term]
id: CIO:0000001
name: confidence statement from single evidence
def: "A confidence information statement defined from a single evidence." [Bgee:fbb]
is_a: CIO:0000000 ! confidence information statement
intersection_of: CIO:0000000 ! confidence information statement
intersection_of: has_evidence_concordance CIO:0000042 {all_only="true"} ! single evidence
intersection_of: has_evidence_type_concordance CIO:0000041 {cardinality="0"} ! evidence type concordance
disjoint_from: CIO:0000002 ! confidence statement from multiple evidence lines
relationship: has_evidence_concordance CIO:0000042 ! single evidence
relationship: has_evidence_type_concordance CIO:0000041 {cardinality="0"} ! evidence type concordance

[Term]
id: CIO:0000002
name: confidence statement from multiple evidence lines
def: "A confidence information statement defined from a set of evidence lines." [Bgee:fbb]
is_a: CIO:0000000 ! confidence information statement
intersection_of: CIO:0000000 ! confidence information statement
intersection_of: has_evidence_concordance CIO:0000043 {all_only="true"} ! concordance of multiple evidence lines
intersection_of: has_evidence_type_concordance CIO:0000041 {cardinality="1"} ! evidence type concordance
relationship: has_evidence_concordance CIO:0000043 ! concordance of multiple evidence lines
relationship: has_evidence_type_concordance CIO:0000041 {cardinality="1"} ! evidence type concordance

[Term]
id: CIO:0000003
name: high confidence from single evidence
def: "A confidence statement from single evidence related to assertions supported by a highly reliable evidence." [Bgee:fbb]
synonym: "gold" RELATED [neXtProt]
is_a: CIO:0000001 ! confidence statement from single evidence
intersection_of: CIO:0000001 ! confidence statement from single evidence
intersection_of: has_confidence_level CIO:0000029 {all_only="true"} ! high confidence level
disjoint_from: CIO:0000004 ! medium confidence from single evidence
disjoint_from: CIO:0000005 ! low confidence from single evidence
disjoint_from: CIO:0000039 ! rejected
relationship: has_confidence_level CIO:0000029 ! high confidence level

[Term]
id: CIO:0000004
name: medium confidence from single evidence
def: "A confidence statement from single evidence related to assertions supported by moderately trusted evidence." [Bgee:fbb]
synonym: "silver" RELATED [neXtProt]
is_a: CIO:0000001 ! confidence statement from single evidence
intersection_of: CIO:0000001 ! confidence statement from single evidence
intersection_of: has_confidence_level CIO:0000030 {all_only="true"} ! medium confidence level
disjoint_from: CIO:0000005 ! low confidence from single evidence
disjoint_from: CIO:0000039 ! rejected
relationship: has_confidence_level CIO:0000030 ! medium confidence level

[Term]
id: CIO:0000005
name: low confidence from single evidence
def: "A confidence statement from single evidence related to assertions supported by not-trusted evidence." [Bgee:fbb]
subset: bgee_not_trusted
synonym: "bronze" RELATED [neXtProt]
is_a: CIO:0000001 ! confidence statement from single evidence
intersection_of: CIO:0000001 ! confidence statement from single evidence
intersection_of: has_confidence_level CIO:0000031 {all_only="true"} ! low confidence level
disjoint_from: CIO:0000039 ! rejected
relationship: has_confidence_level CIO:0000031 ! low confidence level

[Term]
id: CIO:0000006
name: confidence statement from multiple evidence lines of same type
def: "A confidence statement from multiple evidence lines, all using a same experimental or computational type." [Bgee:fbb]
is_a: CIO:0000002 ! confidence statement from multiple evidence lines
intersection_of: CIO:0000002 ! confidence statement from multiple evidence lines
intersection_of: has_evidence_type_concordance CIO:0000037 {all_only="true"} ! same type
disjoint_from: CIO:0000007 ! confidence statement from multiple evidence lines of multiple types
relationship: has_evidence_type_concordance CIO:0000037 ! same type

[Term]
id: CIO:0000007
name: confidence statement from multiple evidence lines of multiple types
def: "A confidence statement from multiple evidence lines, of different experimental or computational types." [Bgee:fbb]
is_a: CIO:0000002 ! confidence statement from multiple evidence lines
intersection_of: CIO:0000002 ! confidence statement from multiple evidence lines
intersection_of: has_evidence_type_concordance CIO:0000038 {all_only="true"} ! different type
relationship: has_evidence_type_concordance CIO:0000038 ! different type

[Term]
id: CIO:0000008
name: confidence statement from congruent evidence lines of multiple types
def: "A confidence statement from multiple evidence lines of multiple types, that are all congruent." [Bgee:fbb]
is_a: CIO:0000007 ! confidence statement from multiple evidence lines of multiple types
intersection_of: CIO:0000007 ! confidence statement from multiple evidence lines of multiple types
intersection_of: has_evidence_concordance CIO:0000033 {all_only="true"} ! congruent
disjoint_from: CIO:0000009 ! confidence statement from conflicting evidence lines of multiple types
relationship: has_evidence_concordance CIO:0000033 ! congruent

[Term]
id: CIO:0000009
name: confidence statement from conflicting evidence lines of multiple types
def: "A confidence statement from multiple evidence lines of multiple types, some of which being contradictory." [Bgee:fbb]
is_a: CIO:0000007 ! confidence statement from multiple evidence lines of multiple types
intersection_of: CIO:0000007 ! confidence statement from multiple evidence lines of multiple types
intersection_of: has_evidence_concordance CIO:0000034 {all_only="true"} ! conflicting
relationship: has_evidence_concordance CIO:0000034 ! conflicting

[Term]
id: CIO:0000010
name: confidence statement from strongly conflicting evidence lines of multiple types
def: "A confidence statement from conflicting evidence lines of multiple types, where evidence lines are in strong contradiction, meaning that the supporting evidence lines yield different conclusion, several of them being equally likely to be true." [Bgee:fbb]
subset: bgee_not_trusted
is_a: CIO:0000009 ! confidence statement from conflicting evidence lines of multiple types
intersection_of: CIO:0000009 ! confidence statement from conflicting evidence lines of multiple types
intersection_of: has_confidence_level CIO:0000028 {cardinality="0"} ! confidence level
intersection_of: has_evidence_concordance CIO:0000035 {all_only="true"} ! strongly conflicting
disjoint_from: CIO:0000011 ! confidence statement from weakly conflicting evidence lines of multiple types
relationship: has_confidence_level CIO:0000028 {cardinality="0"} ! confidence level
relationship: has_evidence_concordance CIO:0000035 ! strongly conflicting

[Term]
id: CIO:0000011
name: confidence statement from weakly conflicting evidence lines of multiple types
def: "A confidence statement from conflicting evidence lines of multiple types, where evidence lines are in weak contradiction, meaning that the overall supported assertion is believed to be true, but a subset of less-reliable evidence lines are in contradiction." [Bgee:fbb]
is_a: CIO:0000009 ! confidence statement from conflicting evidence lines of multiple types
intersection_of: CIO:0000009 ! confidence statement from conflicting evidence lines of multiple types
intersection_of: has_evidence_concordance CIO:0000036 {all_only="true"} ! weakly conflicting
relationship: has_evidence_concordance CIO:0000036 ! weakly conflicting

[Term]
id: CIO:0000012
name: confidence statement from congruent evidence lines of multiple types, overall confidence high
def: "A confidence statement from congruent evidence lines of multiple types, of an overall high confidence level." [Bgee:fbb]
comment: Different strategies can be used to define the overall confidence level: for instance, it could be defined based on the confidence level of the most trusted evidence, from the set of evidence lines supporting the assertion; or, it could be defined based on the number of evidence lines supporting the assertion (e.g., 10 congruent low-confidence evidence lines could allow to have an overall high confidence in an assertion). It is the responsibility of annotation teams to define and communicate the parameters, pertinent to their field, allowing to produce overall confidence levels.
is_a: CIO:0000008 ! confidence statement from congruent evidence lines of multiple types
intersection_of: CIO:0000008 ! confidence statement from congruent evidence lines of multiple types
intersection_of: has_confidence_level CIO:0000029 {all_only="true"} ! high confidence level
disjoint_from: CIO:0000013 ! confidence statement from congruent evidence lines of multiple types, overall confidence medium
disjoint_from: CIO:0000014 ! confidence statement from congruent evidence lines of multiple types, overall confidence low
relationship: has_confidence_level CIO:0000029 ! high confidence level

[Term]
id: CIO:0000013
name: confidence statement from congruent evidence lines of multiple types, overall confidence medium
def: "A confidence statement from congruent evidence lines of multiple types, of an overall moderately trusted confidence level." [Bgee:fbb]
comment: Different strategies can be used to define the overall confidence level: for instance, it could be defined based on the confidence level of the most trusted evidence, from the set of evidence lines supporting the assertion; or, it could be defined based on the number of evidence lines supporting the assertion (e.g., 10 congruent low-confidence evidence lines could allow to have an overall high confidence in an assertion). It is the responsibility of annotation teams to define and communicate the parameters, pertinent to their field, allowing to produce overall confidence levels.
is_a: CIO:0000008 ! confidence statement from congruent evidence lines of multiple types
intersection_of: CIO:0000008 ! confidence statement from congruent evidence lines of multiple types
intersection_of: has_confidence_level CIO:0000030 {all_only="true"} ! medium confidence level
disjoint_from: CIO:0000014 ! confidence statement from congruent evidence lines of multiple types, overall confidence low
relationship: has_confidence_level CIO:0000030 ! medium confidence level

[Term]
id: CIO:0000014
name: confidence statement from congruent evidence lines of multiple types, overall confidence low
def: "A confidence statement from congruent evidence lines of multiple types, of an overall not-trusted confidence level." [Bgee:fbb]
comment: Different strategies can be used to define the overall confidence level: for instance, it could be defined based on the confidence level of the most trusted evidence, from the set of evidence lines supporting the assertion; or, it could be defined based on the number of evidence lines supporting the assertion (e.g., 10 congruent low-confidence evidence lines could allow to have an overall high confidence in an assertion). It is the responsibility of annotation teams to define and communicate the parameters, pertinent to their field, allowing to produce overall confidence levels.
is_a: CIO:0000008 ! confidence statement from congruent evidence lines of multiple types
intersection_of: CIO:0000008 ! confidence statement from congruent evidence lines of multiple types
intersection_of: has_confidence_level CIO:0000031 {all_only="true"} ! low confidence level
relationship: has_confidence_level CIO:0000031 ! low confidence level

[Term]
id: CIO:0000015
name: confidence statement from conflicting evidence lines of same type
def: "Confidence statement from multiple evidence lines of same type, some of which being contradictory." [Bgee:fbb]
is_a: CIO:0000006 ! confidence statement from multiple evidence lines of same type
intersection_of: CIO:0000006 ! confidence statement from multiple evidence lines of same type
intersection_of: has_evidence_concordance CIO:0000034 {all_only="true"} ! conflicting
disjoint_from: CIO:0000016 ! confidence statement from congruent evidence lines of same type
relationship: has_evidence_concordance CIO:0000034 ! conflicting

[Term]
id: CIO:0000016
name: confidence statement from congruent evidence lines of same type
def: "Confidence statement from multiple evidence lines of same type, that are all congruent." [Bgee:fbb]
is_a: CIO:0000006 ! confidence statement from multiple evidence lines of same type
intersection_of: CIO:0000006 ! confidence statement from multiple evidence lines of same type
intersection_of: has_evidence_concordance CIO:0000033 {all_only="true"} ! congruent
relationship: has_evidence_concordance CIO:0000033 ! congruent

[Term]
id: CIO:0000017
name: confidence statement from congruent evidence lines of same type, overall confidence high
def: "A confidence statement from congruent evidence lines of same type, of an overall high confidence level." [Bgee:fbb]
comment: Different strategies can be used to define the overall confidence level: for instance, it could be defined based on the confidence level of the most trusted evidence, from the set of evidence lines supporting the assertion; or, it could be defined based on the number of evidence lines supporting the assertion (e.g., 10 congruent low-confidence evidence lines could allow to have an overall high confidence in an assertion). It is the responsibility of annotation teams to define and communicate the parameters, pertinent to their field, allowing to produce overall confidence levels.
is_a: CIO:0000016 ! confidence statement from congruent evidence lines of same type
intersection_of: CIO:0000016 ! confidence statement from congruent evidence lines of same type
intersection_of: has_confidence_level CIO:0000029 {all_only="true"} ! high confidence level
disjoint_from: CIO:0000018 ! confidence statement from congruent evidence lines of same type, overall confidence low
disjoint_from: CIO:0000019 ! confidence statement from congruent evidence lines of same type, overall confidence medium
relationship: has_confidence_level CIO:0000029 ! high confidence level

[Term]
id: CIO:0000018
name: confidence statement from congruent evidence lines of same type, overall confidence low
def: "A confidence statement from congruent evidence lines of same type, of an overall not-trusted confidence level." [Bgee:fbb]
comment: Different strategies can be used to define the overall confidence level: for instance, it could be defined based on the confidence level of the most trusted evidence, from the set of evidence lines supporting the assertion; or, it could be defined based on the number of evidence lines supporting the assertion (e.g., 10 congruent low-confidence evidence lines could allow to have an overall high confidence in an assertion). It is the responsibility of annotation teams to define and communicate the parameters, pertinent to their field, allowing to produce overall confidence levels.
is_a: CIO:0000016 ! confidence statement from congruent evidence lines of same type
intersection_of: CIO:0000016 ! confidence statement from congruent evidence lines of same type
intersection_of: has_confidence_level CIO:0000031 {all_only="true"} ! low confidence level
disjoint_from: CIO:0000019 ! confidence statement from congruent evidence lines of same type, overall confidence medium
relationship: has_confidence_level CIO:0000031 ! low confidence level

[Term]
id: CIO:0000019
name: confidence statement from congruent evidence lines of same type, overall confidence medium
def: "A confidence statement from congruent evidence lines of same type, of an overall moderately trusted confidence level." [Bgee:fbb]
comment: Different strategies can be used to define the overall confidence level: for instance, it could be defined based on the confidence level of the most trusted evidence, from the set of evidence lines supporting the assertion; or, it could be defined based on the number of evidence lines supporting the assertion (e.g., 10 congruent low-confidence evidence lines could allow to have an overall high confidence in an assertion). It is the responsibility of annotation teams to define and communicate the parameters, pertinent to their field, allowing to produce overall confidence levels.
is_a: CIO:0000016 ! confidence statement from congruent evidence lines of same type
intersection_of: CIO:0000016 ! confidence statement from congruent evidence lines of same type
intersection_of: has_confidence_level CIO:0000030 {all_only="true"} ! medium confidence level
relationship: has_confidence_level CIO:0000030 ! medium confidence level

[Term]
id: CIO:0000020
name: confidence statement from strongly conflicting evidence lines of same type
def: "Confidence statement from conflicting evidence lines of same type, where evidence lines are in strong contradiction, meaning that the supporting evidence lines yield different conclusion, several of them being equally likely to be true." [Bgee:fbb]
subset: bgee_not_trusted
is_a: CIO:0000015 ! confidence statement from conflicting evidence lines of same type
intersection_of: CIO:0000015 ! confidence statement from conflicting evidence lines of same type
intersection_of: has_confidence_level CIO:0000028 {cardinality="0"} ! confidence level
intersection_of: has_evidence_concordance CIO:0000035 {all_only="true"} ! strongly conflicting
disjoint_from: CIO:0000021 ! confidence statement from weakly conflicting evidence lines of same type
relationship: has_confidence_level CIO:0000028 {cardinality="0"} ! confidence level
relationship: has_evidence_concordance CIO:0000035 ! strongly conflicting

[Term]
id: CIO:0000021
name: confidence statement from weakly conflicting evidence lines of same type
def: "Confidence statement from conflicting evidence lines of same type, where evidence lines are in weak contradiction, meaning that the overall supported assertion is believed to be true, but a subset of less-reliable evidence lines are in contradiction." [Bgee:fbb]
is_a: CIO:0000015 ! confidence statement from conflicting evidence lines of same type
intersection_of: CIO:0000015 ! confidence statement from conflicting evidence lines of same type
intersection_of: has_evidence_concordance CIO:0000036 {all_only="true"} ! weakly conflicting
relationship: has_evidence_concordance CIO:0000036 ! weakly conflicting

[Term]
id: CIO:0000022
name: confidence statement from weakly conflicting evidence lines of same type, overall confidence high
def: "Confidence statement from weakly conflicting evidence lines of same type, of an overall high confidence level." [Bgee:fbb]
comment: Different strategies can be used to define the overall confidence level: for instance, it could be defined based on the confidence level of the most trusted evidence, from the set of evidence lines supporting (not contradicting) the assertion; or, it could be defined based on the number of evidence lines supporting the assertion (e.g., 10 congruent low-confidence evidence lines could allow to have an overall high confidence in an assertion, even if contradicted by one other low-confidence evidence). It is the responsibility of annotation teams to define and communicate the parameters, pertinent to their field, allowing to produce overall confidence levels.
is_a: CIO:0000021 ! confidence statement from weakly conflicting evidence lines of same type
intersection_of: CIO:0000021 ! confidence statement from weakly conflicting evidence lines of same type
intersection_of: has_confidence_level CIO:0000029 {all_only="true"} ! high confidence level
disjoint_from: CIO:0000023 ! confidence statement from weakly conflicting evidence lines of same type, overall confidence low
disjoint_from: CIO:0000024 ! confidence statement from weakly conflicting evidence lines of same type, overall confidence medium
relationship: has_confidence_level CIO:0000029 ! high confidence level

[Term]
id: CIO:0000023
name: confidence statement from weakly conflicting evidence lines of same type, overall confidence low
def: "Confidence statement from weakly conflicting evidence lines of same type, of an overall not-trusted confidence level." [Bgee:fbb]
comment: Different strategies can be used to define the overall confidence level: for instance, it could be defined based on the confidence level of the most trusted evidence, from the set of evidence lines supporting (not contradicting) the assertion; or, it could be defined based on the number of evidence lines supporting the assertion (e.g., 10 congruent low-confidence evidence lines could allow to have an overall high confidence in an assertion, even if contradicted by one other low-confidence evidence). It is the responsibility of annotation teams to define and communicate the parameters, pertinent to their field, allowing to produce overall confidence levels.
subset: bgee_not_trusted
is_a: CIO:0000021 ! confidence statement from weakly conflicting evidence lines of same type
intersection_of: CIO:0000021 ! confidence statement from weakly conflicting evidence lines of same type
intersection_of: has_confidence_level CIO:0000031 {all_only="true"} ! low confidence level
disjoint_from: CIO:0000024 ! confidence statement from weakly conflicting evidence lines of same type, overall confidence medium
relationship: has_confidence_level CIO:0000031 ! low confidence level

[Term]
id: CIO:0000024
name: confidence statement from weakly conflicting evidence lines of same type, overall confidence medium
def: "Confidence statement from weakly conflicting evidence lines of same type, of an overall moderately trusted confidence level." [Bgee:fbb]
comment: Different strategies can be used to define the overall confidence level: for instance, it could be defined based on the confidence level of the most trusted evidence, from the set of evidence lines supporting (not contradicting) the assertion; or, it could be defined based on the number of evidence lines supporting the assertion (e.g., 10 congruent low-confidence evidence lines could allow to have an overall high confidence in an assertion, even if contradicted by one other low-confidence evidence). It is the responsibility of annotation teams to define and communicate the parameters, pertinent to their field, allowing to produce overall confidence levels.
is_a: CIO:0000021 ! confidence statement from weakly conflicting evidence lines of same type
intersection_of: CIO:0000021 ! confidence statement from weakly conflicting evidence lines of same type
intersection_of: has_confidence_level CIO:0000030 {all_only="true"} ! medium confidence level
relationship: has_confidence_level CIO:0000030 ! medium confidence level

[Term]
id: CIO:0000025
name: confidence statement from weakly conflicting evidence lines of multiple types, overall confidence high
def: "Confidence statement from weakly conflicting evidence lines of multiple types, of an overall high confidence level." [Bgee:fbb]
comment: Different strategies can be used to define the overall confidence level: for instance, it could be defined based on the confidence level of the most trusted evidence, from the set of evidence lines supporting (not contradicting) the assertion; or, it could be defined based on the number of evidence lines supporting the assertion (e.g., 10 congruent low-confidence evidence lines could allow to have an overall high confidence in an assertion, even if contradicted by one other low-confidence evidence). It is the responsibility of annotation teams to define and communicate the parameters, pertinent to their field, allowing to produce overall confidence levels.
is_a: CIO:0000011 ! confidence statement from weakly conflicting evidence lines of multiple types
intersection_of: CIO:0000011 ! confidence statement from weakly conflicting evidence lines of multiple types
intersection_of: has_confidence_level CIO:0000029 {all_only="true"} ! high confidence level
disjoint_from: CIO:0000026 ! confidence statement from weakly conflicting evidence lines of multiple types, overall confidence low
disjoint_from: CIO:0000027 ! confidence statement from weakly conflicting evidence lines of multiple types, overall confidence medium
relationship: has_confidence_level CIO:0000029 ! high confidence level

[Term]
id: CIO:0000026
name: confidence statement from weakly conflicting evidence lines of multiple types, overall confidence low
def: "Confidence statement from weakly conflicting evidence lines of multiple types, of an overall not-trusted confidence level." [Bgee:fbb]
comment: Different strategies can be used to define the overall confidence level: for instance, it could be defined based on the confidence level of the most trusted evidence, from the set of evidence lines supporting (not contradicting) the assertion; or, it could be defined based on the number of evidence lines supporting the assertion (e.g., 10 congruent low-confidence evidence lines could allow to have an overall high confidence in an assertion, even if contradicted by one other low-confidence evidence). It is the responsibility of annotation teams to define and communicate the parameters, pertinent to their field, allowing to produce overall confidence levels.
subset: bgee_not_trusted
is_a: CIO:0000011 ! confidence statement from weakly conflicting evidence lines of multiple types
intersection_of: CIO:0000011 ! confidence statement from weakly conflicting evidence lines of multiple types
intersection_of: has_confidence_level CIO:0000031 {all_only="true"} ! low confidence level
disjoint_from: CIO:0000027 ! confidence statement from weakly conflicting evidence lines of multiple types, overall confidence medium
relationship: has_confidence_level CIO:0000031 ! low confidence level

[Term]
id: CIO:0000027
name: confidence statement from weakly conflicting evidence lines of multiple types, overall confidence medium
def: "Confidence statement from weakly conflicting evidence lines of multiple types, of an overall moderately trusted confidence level." [Bgee:fbb]
comment: Different strategies can be used to define the overall confidence level: for instance, it could be defined based on the confidence level of the most trusted evidence, from the set of evidence lines supporting (not contradicting) the assertion; or, it could be defined based on the number of evidence lines supporting the assertion (e.g., 10 congruent low-confidence evidence lines could allow to have an overall high confidence in an assertion, even if contradicted by one other low-confidence evidence). It is the responsibility of annotation teams to define and communicate the parameters, pertinent to their field, allowing to produce overall confidence levels.
is_a: CIO:0000011 ! confidence statement from weakly conflicting evidence lines of multiple types
intersection_of: CIO:0000011 ! confidence statement from weakly conflicting evidence lines of multiple types
intersection_of: has_confidence_level CIO:0000030 {all_only="true"} ! medium confidence level
relationship: has_confidence_level CIO:0000030 ! medium confidence level

[Term]
id: CIO:0000028
name: confidence level
def: "A confidence information element representing the different levels of confidence, used to compose confidence information statements." [Bgee:fbb]
is_a: CIO:0000040 ! confidence information element
disjoint_from: CIO:0000032 ! evidence concordance
disjoint_from: CIO:0000041 ! evidence type concordance

[Term]
id: CIO:0000029
name: high confidence level
def: "A confidence level representing a high trust in an evidence." [Bgee:fbb]
is_a: CIO:0000028 ! confidence level
disjoint_from: CIO:0000030 ! medium confidence level
disjoint_from: CIO:0000031 ! low confidence level
relationship: provides_greater_confidence_than CIO:0000030 ! medium confidence level

[Term]
id: CIO:0000030
name: medium confidence level
def: "A confidence level representing a moderate trust in an evidence." [Bgee:fbb]
is_a: CIO:0000028 ! confidence level
disjoint_from: CIO:0000031 ! low confidence level
relationship: provides_greater_confidence_than CIO:0000031 ! low confidence level

[Term]
id: CIO:0000031
name: low confidence level
def: "A confidence level representing an absence of trust in an evidence." [Bgee:fbb]
is_a: CIO:0000028 ! confidence level

[Term]
id: CIO:0000032
name: evidence concordance
def: "A confidence information element representing the type of concordance of evidence lines supporting an assertion, used to compose confidence information statements." [Bgee:fbb]
comment: Subclasses are used to define whether there is a single evidence, or multiple evidence lines, in support of an assertion, and whether they are congruent or conflicting.
is_a: CIO:0000040 ! confidence information element
disjoint_from: CIO:0000041 ! evidence type concordance

[Term]
id: CIO:0000033
name: congruent
def: "An evidence concordance of multiple evidence lines that are congruent." [Bgee:fbb]
comment: The assumption here is that assertions supported by a single evidence are less trustworthy than assertions supported by multiple evidence lines.
is_a: CIO:0000043 ! concordance of multiple evidence lines
disjoint_from: CIO:0000034 ! conflicting

[Term]
id: CIO:0000034
name: conflicting
def: "An evidence concordance of multiple evidence lines that are conflicting." [Bgee:fbb]
comment: An assertion can have several related evidence lines, some supporting the assertion, and some rejecting the assertion (e.g., using the NOT qualifier in GO annotations).
is_a: CIO:0000043 ! concordance of multiple evidence lines

[Term]
id: CIO:0000035
name: strongly conflicting
def: "A conflicting concordance for evidence lines that are strongly conflicting." [Bgee:fbb]
comment: We distinguish two levels of conflict: weak conflict between evidence lines, e.g., a low confidence evidence negating an assertion, versus several high confidence evidence lines supporting the assertion; and strong conflict between evidence lines, e.g., two high confidence evidence lines contradicting each other. Note that strongly conflicting evidence lines are not used to produce confidence information statements associated to a confidence level (low, medium, high): in that case, the supported assertion is believed to need further validation, as evidence lines yield different conclusions of similar confidence.
is_a: CIO:0000034 ! conflicting
disjoint_from: CIO:0000036 ! weakly conflicting

[Term]
id: CIO:0000036
name: weakly conflicting
def: "A conflicting concordance for evidence lines that are weakly conflicting." [Bgee:fbb]
comment: We distinguish two levels of conflict: weak conflict between evidence lines, e.g., a low confidence evidence negating an assertion, versus several high confidence evidence lines supporting the assertion; and strong conflict between evidence lines, e.g., two high confidence evidence lines contradicting each other.
is_a: CIO:0000034 ! conflicting

[Term]
id: CIO:0000037
name: same type
def: "An evidence type concordance for evidence lines that are from a same type." [Bgee:fbb]
is_a: CIO:0000041 ! evidence type concordance
disjoint_from: CIO:0000038 ! different type

[Term]
id: CIO:0000038
name: different type
def: "An evidence type concordance for evidence lines that are from different types." [Bgee:fbb]
is_a: CIO:0000041 ! evidence type concordance

[Term]
id: CIO:0000039
name: rejected
def: "A confidence statement from single evidence related to assertions that have been rejected, for instance, following paper retraction, author misinterpretation, or curator misinterpretation." [Bgee:fbb]
comment: When results are retracted, associated annotations are often removed. Consequently, end-users might not be aware that the result was annotated. Annotating an assertion with this confidence term allows to keep the information available. Such assertions should not interfer with aggregation of multiple evidence lines to generate a confidence level from the branch CIO:0000002 "confidence from multiple evidence lines". This is different from negative annotations, used to negate the interpretation of an annotation. It is also different from conflicting multiple evidence lines, where each single evidence has not been directly invalidated. Rejection is a stronger assertion about an annotation source than conflict, capturing that this evidence should no longer be used.
is_a: CIO:0000001 ! confidence statement from single evidence

[Term]
id: CIO:0000040
name: confidence information element
def: "Confidence information element represent intrinsic properties of confidence information statements, allowing to compose them." [Bgee:fbb]

[Term]
id: CIO:0000041
name: evidence type concordance
def: "A confidence information element representing the concordance of experimental or computational types of evidence lines supporting an assertion, used to compose confidence information statements." [Bgee:fbb]
comment: The assumption here is that assertions supported by evidence lines of different experimental or computational types are more trustworthy than assertions supported by evidence lines of a same experimental or computational type.
is_a: CIO:0000040 ! confidence information element

[Term]
id: CIO:0000042
name: single evidence
def: "An evidence concordance for confidence information about an assertion produced from a single evidence." [Bgee:fbb]
comment: The assumption here is that assertions supported by a single evidence are less trustworthy than assertions supported by multiple evidence lines.
is_a: CIO:0000032 ! evidence concordance
disjoint_from: CIO:0000043 ! concordance of multiple evidence lines

[Term]
id: CIO:0000043
name: concordance of multiple evidence lines
def: "An evidence concordance for confidence information about an assertion produced from multiple evidence lines." [Bgee:fbb]
comment: The assumption here is that assertions supported by a single evidence are less trustworthy than assertions supported by multiple evidence lines.
is_a: CIO:0000032 ! evidence concordance

[Typedef]
id: has_confidence_element
name: has confidence element
def: "X has confidence element Y iff X is a confidence information statement and Y is an associated confidence information element, used to define the statement." []
domain: CIO:0000000 ! confidence information statement
range: CIO:0000040 ! confidence information element

[Typedef]
id: has_confidence_level
name: has confidence level
def: "X has confidence level Y iff X is a confidence information statement and Y is it associated confidence information level." []
range: CIO:0000028 ! confidence level
is_a: has_confidence_element ! has confidence element

[Typedef]
id: has_evidence_concordance
name: has evidence concordance
def: "X has evidence concordance Y iff X is a confidence information statement and Y is it associated evidence concordance." []
domain: CIO:0000000 ! confidence information statement
range: CIO:0000032 ! evidence concordance
is_a: has_confidence_element ! has confidence element

[Typedef]
id: has_evidence_type_concordance
name: has evidence type concordance
def: "X has evidence type concordance Y iff X is a confidence information statement and Y is it associated evidence type concordance." []
range: CIO:0000041 ! evidence type concordance
is_a: has_confidence_element ! has confidence element

[Typedef]
id: provides_greater_confidence_than
name: provides greater confidence than
def: "X provides greater confidence than Y iff both X and Y provide a confidence information level, and the level of confidence provided by X is greater than the level of confidence provided by Y." []
domain: CIO:0000028 ! confidence level
range: CIO:0000028 ! confidence level
is_transitive: true

