format-version: 1.2
data-version: releases/2015-01-24
ontology: confidence_information_ontology

[Term]
id: CIO:0000000
name: confidence information statement
def: "A statement providing information about the confidence in an assertion, meaning, an information about the level of certainty that an assertion is correct." [Bgee]
comment: Quality and confidence are distinct concepts: quality refers to the value of a source or of an annotation, whereas confidence refers to the level of certainty that an assertion is correct.

[Term]
id: CIO:0000001
name: confidence from single evidence
def: "A confidence information about an assertion, defined from a single evidence." [Bgee:draft]
is_a: CIO:0000000 ! confidence information statement
intersection_of: CIO:0000000 ! confidence information statement
intersection_of: CIO:0000042 ! single evidence
disjoint_from: CIO:0000002 ! confidence from multiple evidence lines

[Term]
id: CIO:0000002
name: confidence from multiple evidence lines
def: "A confidence information about an assertion, defined from a set of evidence lines." [Bgee:draft]
is_a: CIO:0000000 ! confidence information statement
intersection_of: CIO:0000000 ! confidence information statement
intersection_of: CIO:0000043 ! concordance of multiple evidence lines

[Term]
id: CIO:0000003
name: high confidence from single evidence
def: "A confidence information related to assertions supported by a highly reliable evidence." [Bgee:draft]
synonym: "gold" RELATED [neXtProt]
is_a: CIO:0000001 ! confidence from single evidence
intersection_of: CIO:0000001 ! confidence from single evidence
intersection_of: CIO:0000029 ! high confidence level
disjoint_from: CIO:0000004 ! medium confidence from single evidence
disjoint_from: CIO:0000005 ! low confidence from single evidence
disjoint_from: CIO:0000039 ! rejected

[Term]
id: CIO:0000004
name: medium confidence from single evidence
def: "A confidence information related to assertions supported by moderately trusted evidence." [Bgee:draft]
synonym: "silver" RELATED [neXtProt]
is_a: CIO:0000001 ! confidence from single evidence
intersection_of: CIO:0000001 ! confidence from single evidence
intersection_of: CIO:0000030 ! medium confidence level
disjoint_from: CIO:0000005 ! low confidence from single evidence
disjoint_from: CIO:0000039 ! rejected

[Term]
id: CIO:0000005
name: low confidence from single evidence
def: "A confidence information related to assertions supported by not-trusted evidence." [Bgee:draft]
synonym: "bronze" RELATED [neXtProt]
is_a: CIO:0000001 ! confidence from single evidence
intersection_of: CIO:0000001 ! confidence from single evidence
intersection_of: CIO:0000031 ! low confidence level
disjoint_from: CIO:0000039 ! rejected

[Term]
id: CIO:0000006
name: confidence from multiple evidence lines of same type
def: "A confidence from multiple evidence lines, all using a same type." [Bgee:draft]
is_a: CIO:0000002 ! confidence from multiple evidence lines
intersection_of: CIO:0000002 ! confidence from multiple evidence lines
intersection_of: CIO:0000037 ! same type
disjoint_from: CIO:0000007 ! confidence from multiple evidence lines of multiple types

[Term]
id: CIO:0000007
name: confidence from multiple evidence lines of multiple types
def: "A confidence from multiple evidence lines, using different types." [Bgee:draft]
is_a: CIO:0000002 ! confidence from multiple evidence lines
intersection_of: CIO:0000002 ! confidence from multiple evidence lines
intersection_of: CIO:0000038 ! different type

[Term]
id: CIO:0000008
name: confidence from congruent evidence lines of multiple types
def: "A confidence from multiple evidence lines, that are all congruent." [Bgee:draft]
is_a: CIO:0000007 ! confidence from multiple evidence lines of multiple types
intersection_of: CIO:0000007 ! confidence from multiple evidence lines of multiple types
intersection_of: CIO:0000033 ! congruent
disjoint_from: CIO:0000009 ! confidence from conflicting evidence lines of multiple types

[Term]
id: CIO:0000009
name: confidence from conflicting evidence lines of multiple types
def: "A confidence from multiple evidence lines, some of which being contradictory." [Bgee:draft]
is_a: CIO:0000007 ! confidence from multiple evidence lines of multiple types
intersection_of: CIO:0000007 ! confidence from multiple evidence lines of multiple types
intersection_of: CIO:0000034 ! conflicting

[Term]
id: CIO:0000010
name: confidence from strongly conflicting evidence lines of multiple types
def: "Conflicting evidence lines of multiple types in strong contradiction, meaning that the supporting evidence lines yield different conclusion, several of them being equally likely to be true." [Bgee:draft]
is_a: CIO:0000009 ! confidence from conflicting evidence lines of multiple types
intersection_of: CIO:0000009 ! confidence from conflicting evidence lines of multiple types
intersection_of: CIO:0000035 ! strongly conflicting
disjoint_from: CIO:0000011 ! confidence from weakly conflicting evidence lines of multiple types

[Term]
id: CIO:0000011
name: confidence from weakly conflicting evidence lines of multiple types
def: "Conflicting evidence lines in weak contradiction, meaning that the overall supported assertion is believed to be true, but a subset of less-reliable evidence lines are in contradiction." [Bgee:draft]
is_a: CIO:0000009 ! confidence from conflicting evidence lines of multiple types
intersection_of: CIO:0000009 ! confidence from conflicting evidence lines of multiple types
intersection_of: CIO:0000036 ! weakly conflicting

[Term]
id: CIO:0000012
name: confidence from congruent evidence lines of multiple types, best confidence high
def: "Congruent evidence lines, the best supporting evidence being a highly reliable evidence." [Bgee:draft]
is_a: CIO:0000008 ! confidence from congruent evidence lines of multiple types
intersection_of: CIO:0000008 ! confidence from congruent evidence lines of multiple types
intersection_of: CIO:0000029 ! high confidence level
disjoint_from: CIO:0000013 ! confidence from congruent evidence lines of multiple types, best confidence medium
disjoint_from: CIO:0000014 ! confidence from congruent evidence lines of multiple types, best confidence low

[Term]
id: CIO:0000013
name: confidence from congruent evidence lines of multiple types, best confidence medium
def: "Congruent evidence lines, the best supporting evidence being a moderately trusted evidence." [Bgee:draft]
is_a: CIO:0000008 ! confidence from congruent evidence lines of multiple types
intersection_of: CIO:0000008 ! confidence from congruent evidence lines of multiple types
intersection_of: CIO:0000030 ! medium confidence level
disjoint_from: CIO:0000014 ! confidence from congruent evidence lines of multiple types, best confidence low

[Term]
id: CIO:0000014
name: confidence from congruent evidence lines of multiple types, best confidence low
def: "Congruent evidence lines, the best supporting evidence being a not-trusted evidence." [Bgee:draft]
is_a: CIO:0000008 ! confidence from congruent evidence lines of multiple types
intersection_of: CIO:0000008 ! confidence from congruent evidence lines of multiple types
intersection_of: CIO:0000031 ! low confidence level

[Term]
id: CIO:0000015
name: confidence from conflicting evidence lines of same type
def: "Confidence from multiple evidence lines of same type, some of which being contradictory." [Bgee:draft]
is_a: CIO:0000006 ! confidence from multiple evidence lines of same type
intersection_of: CIO:0000006 ! confidence from multiple evidence lines of same type
intersection_of: CIO:0000034 ! conflicting
disjoint_from: CIO:0000016 ! confidence from congruent evidence lines of same type

[Term]
id: CIO:0000016
name: confidence from congruent evidence lines of same type
def: "Confidence from multiple evidence lines of same type, that are all congruent." [Bgee:draft]
is_a: CIO:0000006 ! confidence from multiple evidence lines of same type
intersection_of: CIO:0000006 ! confidence from multiple evidence lines of same type
intersection_of: CIO:0000033 ! congruent

[Term]
id: CIO:0000017
name: confidence from congruent evidence lines of same type, best confidence high
def: "Congruent evidence lines, the best supporting evidence being a highly reliable evidence." [Bgee:draft]
is_a: CIO:0000016 ! confidence from congruent evidence lines of same type
intersection_of: CIO:0000016 ! confidence from congruent evidence lines of same type
intersection_of: CIO:0000029 ! high confidence level
disjoint_from: CIO:0000018 ! confidence from congruent evidence lines of same type, best confidence low
disjoint_from: CIO:0000019 ! confidence from congruent evidence lines of same type, best confidence medium

[Term]
id: CIO:0000018
name: confidence from congruent evidence lines of same type, best confidence low
def: "Congruent evidence lines, the best supporting evidence being a not-trusted evidence." [Bgee:draft]
is_a: CIO:0000016 ! confidence from congruent evidence lines of same type
intersection_of: CIO:0000016 ! confidence from congruent evidence lines of same type
intersection_of: CIO:0000031 ! low confidence level
disjoint_from: CIO:0000019 ! confidence from congruent evidence lines of same type, best confidence medium

[Term]
id: CIO:0000019
name: confidence from congruent evidence lines of same type, best confidence medium
def: "Congruent evidence lines, the best supporting evidence being a moderately trusted evidence." [Bgee:draft]
is_a: CIO:0000016 ! confidence from congruent evidence lines of same type
intersection_of: CIO:0000016 ! confidence from congruent evidence lines of same type
intersection_of: CIO:0000030 ! medium confidence level

[Term]
id: CIO:0000020
name: confidence from strongly conflicting evidence lines of same type
def: "Conflicting evidence lines in strong contradiction, meaning that the supporting evidence lines yield different conclusion, several of them being equally likely to be true." [Bgee:draft]
is_a: CIO:0000015 ! confidence from conflicting evidence lines of same type
intersection_of: CIO:0000015 ! confidence from conflicting evidence lines of same type
intersection_of: CIO:0000035 ! strongly conflicting
disjoint_from: CIO:0000021 ! confidence from weakly conflicting evidence lines of same type

[Term]
id: CIO:0000021
name: confidence from weakly conflicting evidence lines of same type
def: "Conflicting evidence lines in weak contradiction, meaning that the overall supported assertion is believed to be true, but a subset of less-reliable evidence lines are in contradiction." [Bgee:draft]
is_a: CIO:0000015 ! confidence from conflicting evidence lines of same type
intersection_of: CIO:0000015 ! confidence from conflicting evidence lines of same type
intersection_of: CIO:0000036 ! weakly conflicting

[Term]
id: CIO:0000022
name: confidence from weakly conflicting evidence lines of same type, best confidence high
def: "Weakly conflicting evidence lines, the best supporting evidence from the subset of evidence lines supporting the assertion (not in contradiction) being a highly reliable evidence." [Bgee:draft]
is_a: CIO:0000021 ! confidence from weakly conflicting evidence lines of same type
intersection_of: CIO:0000021 ! confidence from weakly conflicting evidence lines of same type
intersection_of: CIO:0000029 ! high confidence level
disjoint_from: CIO:0000023 ! confidence from weakly conflicting evidence lines of same type, best confidence low
disjoint_from: CIO:0000024 ! confidence from weakly conflicting evidence lines of same type, best confidence medium

[Term]
id: CIO:0000023
name: confidence from weakly conflicting evidence lines of same type, best confidence low
def: "Weakly conflicting evidence lines, the best supporting evidence from the subset of evidence lines supporting the assertion (not in contradiction) being a not-trusted evidence." [Bgee:draft]
is_a: CIO:0000021 ! confidence from weakly conflicting evidence lines of same type
intersection_of: CIO:0000021 ! confidence from weakly conflicting evidence lines of same type
intersection_of: CIO:0000031 ! low confidence level
disjoint_from: CIO:0000024 ! confidence from weakly conflicting evidence lines of same type, best confidence medium

[Term]
id: CIO:0000024
name: confidence from weakly conflicting evidence lines of same type, best confidence medium
def: "Weakly conflicting evidence lines, the best supporting evidence from the subset of evidence lines supporting the assertion (not in contradiction) being a moderately trusted evidence." [Bgee:draft]
is_a: CIO:0000021 ! confidence from weakly conflicting evidence lines of same type
intersection_of: CIO:0000021 ! confidence from weakly conflicting evidence lines of same type
intersection_of: CIO:0000030 ! medium confidence level

[Term]
id: CIO:0000025
name: confidence from weakly conflicting evidence lines of multiple types, best confidence high
def: "Weakly conflicting evidence lines, the best supporting evidence from the subset of evidence lines supporting the assertion (not in contradiction) being a highly reliable evidence." [Bgee:draft]
is_a: CIO:0000011 ! confidence from weakly conflicting evidence lines of multiple types
intersection_of: CIO:0000011 ! confidence from weakly conflicting evidence lines of multiple types
intersection_of: CIO:0000029 ! high confidence level
disjoint_from: CIO:0000026 ! confidence from weakly conflicting evidence lines of multiple types, best confidence low
disjoint_from: CIO:0000027 ! confidence from weakly conflicting evidence lines of multiple types, best confidence medium

[Term]
id: CIO:0000026
name: confidence from weakly conflicting evidence lines of multiple types, best confidence low
def: "Weakly conflicting evidence lines, the best supporting evidence from the subset of evidence lines supporting the assertion (not in contradiction) being a not-trusted evidence." [Bgee:draft]
is_a: CIO:0000011 ! confidence from weakly conflicting evidence lines of multiple types
intersection_of: CIO:0000011 ! confidence from weakly conflicting evidence lines of multiple types
intersection_of: CIO:0000031 ! low confidence level
disjoint_from: CIO:0000027 ! confidence from weakly conflicting evidence lines of multiple types, best confidence medium

[Term]
id: CIO:0000027
name: confidence from weakly conflicting evidence lines of multiple types, best confidence medium
def: "Weakly conflicting evidence lines, the best supporting evidence from the subset of evidence lines supporting the assertion (not in contradiction) being a moderately trusted evidence." [Bgee:draft]
is_a: CIO:0000011 ! confidence from weakly conflicting evidence lines of multiple types
intersection_of: CIO:0000011 ! confidence from weakly conflicting evidence lines of multiple types
intersection_of: CIO:0000030 ! medium confidence level

[Term]
id: CIO:0000028
name: confidence level
def: "A confidence information element representing the different levels of confidence, used to compose confidence information statements." [Bgee:draft]
is_a: CIO:0000040 ! confidence information element

[Term]
id: CIO:0000029
name: high confidence level
def: "A confidence level representing a high trust in an evidence." [Bgee:draft]
is_a: CIO:0000028 ! confidence level
disjoint_from: CIO:0000030 ! medium confidence level
disjoint_from: CIO:0000031 ! low confidence level

[Term]
id: CIO:0000030
name: medium confidence level
def: "A confidence level representing a moderate trust in an evidence." [Bgee:draft]
is_a: CIO:0000028 ! confidence level
disjoint_from: CIO:0000031 ! low confidence level

[Term]
id: CIO:0000031
name: low confidence level
def: "A confidence level representing an absence of trust in an evidence." [Bgee:draft]
is_a: CIO:0000028 ! confidence level

[Term]
id: CIO:0000032
name: evidence concordance
def: "A confidence information element representing the type of concordance of evidence lines supporting an assertion, used to compose confidence information statements." [Bgee:draft]
comment: Subclasses are used to define whether there is a single evidence, or multiple evidence lines, in support of an assertion, and whether they are congruent or conflicting.
is_a: CIO:0000040 ! confidence information element

[Term]
id: CIO:0000033
name: congruent
def: "An evidence concordance of multiple evidence lines that are congruent." [Bgee:draft]
comment: The assumption here is that assertions supported by a single evidence are less trustworthy than assertions supported by multiple evidence lines.
is_a: CIO:0000043 ! concordance of multiple evidence lines
disjoint_from: CIO:0000034 ! conflicting

[Term]
id: CIO:0000034
name: conflicting
def: "An evidence concordance of multiple evidence lines that are conflicting." [Bgee:draft]
comment: An assertion can have several related evidence lines, some supporting the assertion, and some rejecting the assertion (e.g., using the NOT qualifier in GO annotations).
is_a: CIO:0000043 ! concordance of multiple evidence lines

[Term]
id: CIO:0000035
name: strongly conflicting
def: "A conflicting concordance for evidence lines that are strongly conflicting." [Bgee:draft]
comment: We distinguish two levels of conflict: weak conflict between evidence lines, e.g., a low confidence evidence negating an assertion, versus several high confidence evidence lines supporting the assertion; and strong conflict between evidence lines, e.g., two high confidence evidence lines contradicting each other. Note that strongly conflicting evidence lines are not used to produce confidence information statements associated to a confidence level (low, medium, high): in that case, the supported assertion is believed to need further validation, as evidence lines yield different conclusions of similar confidence.
is_a: CIO:0000034 ! conflicting
disjoint_from: CIO:0000036 ! weakly conflicting

[Term]
id: CIO:0000036
name: weakly conflicting
def: "A conflicting concordance for evidence lines that are weakly conflicting." [Bgee:draft]
comment: We distinguish two levels of conflict: weak conflict between evidence lines, e.g., a low confidence evidence negating an assertion, versus several high confidence evidence lines supporting the assertion; and strong conflict between evidence lines, e.g., two high confidence evidence lines contradicting each other.
is_a: CIO:0000034 ! conflicting

[Term]
id: CIO:0000037
name: same type
def: "An evidence type concordance for evidence lines that are from a same type." [Bgee:draft]
is_a: CIO:0000041 ! evidence type concordance
disjoint_from: CIO:0000038 ! different type

[Term]
id: CIO:0000038
name: different type
def: "An evidence type concordance for evidence lines that are from different types." [Bgee:draft]
is_a: CIO:0000041 ! evidence type concordance

[Term]
id: CIO:0000039
name: rejected
def: "A confidence information related to assertions that have been rejected, for instance, following paper retraction, author misinterpretation, or curator misinterpretation." [Bgee:draft]
comment: When results are retracted, associated annotations are often removed. Consequently, end-users might not be aware that the result was annotated. Annotating an assertion with this confidence term allows to keep the information available. Such assertions should not interfer with aggregation of multiple evidence lines to generate a confidence level from the branch CIO:0000002 "confidence from multiple evidence lines". This is different from negative annotations, used to negate the interpretation of an annotation. It is also different from conflicting multiple evidence lines, where each single evidence has not been directly invalidated. Rejection is a stronger assertion about an annotation source than conflict, capturing that this evidence should no longer be used.
is_a: CIO:0000001 ! confidence from single evidence

[Term]
id: CIO:0000040
name: confidence information element
def: "A confidence information element allowing to compose confidence information statements." [Bgee]

[Term]
id: CIO:0000041
name: evidence type concordance
def: "A confidence information element representing the concordance of experimental or computational types of evidence lines supporting an assertion, used to compose confidence information statements." [Bgee]
comment: The assumption here is that assertions supported by evidence lines of different experimental or computational types are more trustworthy than assertions supported by evidence lines of a same experimental or computational type.
is_a: CIO:0000040 ! confidence information element

[Term]
id: CIO:0000042
name: single evidence
def: "An evidence concordance for confidence information about an assertion produced from a single evidence." [Bgee:draft]
comment: The assumption here is that assertions supported by a single evidence are less trustworthy than assertions supported by multiple evidence lines.
is_a: CIO:0000032 ! evidence concordance
disjoint_from: CIO:0000043 ! concordance of multiple evidence lines

[Term]
id: CIO:0000043
name: concordance of multiple evidence lines
def: "An evidence concordance for confidence information about an assertion produced from multiple evidence lines." [Bgee:draft]
comment: The assumption here is that assertions supported by a single evidence are less trustworthy than assertions supported by multiple evidence lines.
is_a: CIO:0000032 ! evidence concordance

